$1+\cos(2\theta)=2\cos^2(\theta)\\
1-\cos(2\theta)=2\sin^2(\theta)\\
\sin(\theta)\cos(\theta)=\frac{1}{2}2\sin(\theta)\cos(\theta)=\frac{1}{2}\sin(2\theta)\\
1-\sin(2\theta)=\sin^2(\theta)+\cos^2(\theta)-2\sin(\theta)\cos(\theta) = (\sin(\theta)-\cos(\theta))^2\\
\sin^6(x)+\cos^6(x)=1-3\sin^2(x)\cos^2(c)\\
\sin^4(x)+\cos^4(x)=1-2\sin^2(x)\cos^2(x)\\
\sin^2(\theta)=\frac{1-\cos(2\theta)}{2}\\
\cos(2x)=\cos^2(x)-\sin^2(x)=2\cos^2(x)-1=1-2\sin^2(x)\\
\sin^2(x)=\frac{1-\cos(2x)}{2}\\
\cos^(x)=\frac{1+\cos(2x)}{2}\\
\sin(A+B)\sin(A-B)=\cos^2(A)-\cos^2(B)\\
\sin(3x)=3\sin(x)-4\sin^3(x)\\
\cos(3x)=4\cos^3(x)-3\cos(x)\\
2\cos(A)\cos(B)=\cos(A+B)+\cos(A-B)\\
2\cos(A)\sin(B)=\sin(A+B)+\sin(A-B)\\
2\sin(A)\sin(B)=\cos(A-B)-\cos(A+B)\\
$